First of all, prove soundness for propositional rules including DNE. Then, the remaining rules to consider are the quantifier rules. \textcolor{Maroon}{\P}\
For $\forall E$, suppose we have $X \Yright \forall x A(x)$. From the inductive hypothesis, $X \vDash_{FO} \forall x A(x)$. We need to prove $\forall x A(x) \vDash_{FO} A(t)$, provided that the term $t$ is free for $x$ in $A(x)$, so to prove $X \vDash_{FO} A(t)$. \textcolor{Maroon}{\P}\
For $\exists I$, suppose we have $X \Yright A(t)$. From the inductive hypothesis, $X \vDash_{FO} A(t)$. We need to prove $A(t) \vDash_{FO} \exists x A(x)$, provided that the term $t$ is free for $x$ in $A(x)$, so to prove $X \vDash_{FO} \exists x A(x)$. \textcolor{Maroon}{\P}\
For $\forall I$, suppose we have $X \Yright A(t)$. From the inductive hypothesis, $X \vDash_{FO} A(t)$. We need to prove $A(t) \vDash_{FO} \forall x A(x)$, provided that the term $t$ is not present in the premises $X$ and is free for $x$ in $A(x)$, so to prove $X \vDash_{FO} \forall x A(x)$. \textcolor{Maroon}{\P}\
For $\exists E$, suppose we have $X \Yright \exists x A(x)$ and $Y, A(t) \Yright C$. From the inductive hypothesis, $X \vDash_{FO} \exists x A(x)$ and $Y, A(t) \vDash_{FO} C$. We need to prove if $X \vDash_{FO} \exists x A(x)$ and $Y, A(t) \vDash_{FO} C$, then $X,Y \vDash_{FO} C$, provided that the term $t$ does not occur in $Y$, $\exists x A(x)$, and C, and $t$ is free for $x$ in $A(x)$.
